pulse/lib/pulse/core/PulseCore.Atomic.fsti
@@ -319,7 +319,7 @@ val later_elim (p:slprop)
 val later_elim_timeless (p:slprop { timeless p })
 : stt_ghost unit emp_inames (later p) (fun _ -> p)
 
-val buy (n:erased nat)
+val buy (n:nat)
 : stt unit emp (fun _ -> later_credit n)
 
 ////////////////////////////////////////////////////////////////////////
